compiler.v
@@ -1,5 +1,5 @@
 Require expr cbn cem cesm im db assembly.
-Require cem_cesm cesm_im.
+Require Import cem_cesm cesm_im.
 Require Import Unicode.Utf8.
 Require Import util expr_db db_assembly relations.
 
@@ -8,9 +8,11 @@ main theorems of correctness *)
 
 Definition compile t := assemble t 0.
 
-Theorem compile_correct (t : db.tm) : db.closed t → cem.step (cem.I t) v → 
-  { mv : im.State | refl_trans_clos im.step (im.I (compile t)) mv *
-                    state_rel (cesm.st mv cem.st_h } 
+Theorem compile_correct (t : db.tm) v : db.closed t → cem.step (cem.I t) v → 
+  { mv : im.State & refl_trans_clos im.step (im.I (compile t)) mv *
+                    state_rel (cesm.st (cem.conf_h v) nil (cem.conf_c v))
+                              mv }.
+Admitted.
 (*Theorem compile_correct : Type := bool.
  Definition compile (t: expr.tm) : expr.closed t → { mc | trans_clos prog p }.
 *)
